wip

code/lib/Hacl.Spec.Endianness.fst
@@ -14,15 +14,42 @@ module H32  = Hacl.UInt32
 module H64  = Hacl.UInt64
 module H128 = Hacl.UInt128
 
-#set-options "--initial_fuel 0 --max_fuel 0 --z3rlimit 5"
+#reset-options "--initial_fuel 1 --max_fuel 1 --z3rlimit 20"
 
 let h8_to_u8 (x:H8.t) : GTot (y:U8.t{U8.v y = H8.v x}) = U8.uint_to_t (H8.v x)
 
-assume val seq_map: #a:Type -> #b:Type -> f:(a -> GTot b) -> s:Seq.seq a ->
+private val seq_map_:
+  #a:Type -> #b:Type ->
+  f:(a -> GTot b) ->
+  s:Seq.seq a ->
+  j:nat{j <= Seq.length s} ->
+  s':Seq.seq b{Seq.length s' = Seq.length s /\ (forall (i:nat). {:pattern (Seq.index s' i)}
+    i < j ==> Seq.index s' i == f (Seq.index s i))} ->
+    GTot (s'':Seq.seq b{Seq.length s'' = Seq.length s
+      /\ (forall (i:nat). {:pattern (Seq.index s'' i)} i < Seq.length s ==> Seq.index s'' i == f (Seq.index s i))})
+  (decreases (Seq.length s - j))
+private let rec seq_map_ #a #b f s j s' =
+  if j = Seq.length s then s'
+  else (
+    let s' = Seq.upd s' j (f (Seq.index s j)) in
+    seq_map_ f s (j+1) s'
+  )
+
+val seq_map: #a:Type -> #b:Type -> f:(a -> GTot b) -> s:Seq.seq a ->
   GTot (s':Seq.seq b{Seq.length s' = Seq.length s /\ (forall (i:nat). i < Seq.length s ==> Seq.index s' i == f (Seq.index s i))})
+let seq_map #a #b f s =
+  if Seq.length s = 0 then Seq.createEmpty #b
+  else seq_map_ f s 0 (Seq.create (Seq.length s) (f (Seq.index s 0)))
+  
 
-inline_for_extraction let hlittle_endian (s:Seq.seq H8.t) : GTot nat =
-  little_endian (seq_map h8_to_u8 s)
+unfold inline_for_extraction
+let reveal_sbytes (s:Seq.seq H8.t) : GTot (s:Seq.seq U8.t) = seq_map h8_to_u8 s
 
-inline_for_extraction let hbig_endian (s:Seq.seq H8.t) : GTot nat =
-  big_endian (seq_map h8_to_u8 s)
+
+unfold inline_for_extraction 
+let hlittle_endian (s:Seq.seq H8.t) : GTot nat =
+  little_endian (reveal_sbytes s)
+
+unfold inline_for_extraction
+let hbig_endian (s:Seq.seq H8.t) : GTot nat =
+  big_endian (reveal_sbytes s)
