code/poly1305/Hacl.Impl.Poly1305_64.fst
@@ -9,7 +9,6 @@ open FStar.HyperStack
 open FStar.Endianness
 open FStar.Buffer
 
-(* open C *)
 open Hacl.Endianness
 
 open Hacl.Cast
@@ -57,7 +56,7 @@ private let live_st m (st:poly1305_state) : Type0 =
 (* ############################################################################# *)
 
 
-#set-options "--z3rlimit 100 --initial_fuel 0 --max_fuel 0"
+#set-options "--z3rlimit 100 --initial_fuel 0 --max_fuel 0 --initial_ifuel 0 --max_ifuel 0"
 
 [@"c_inline"]
 inline_for_extraction val upd_3: b:felem -> b0:limb -> b1:limb -> b2:limb ->
@@ -106,8 +105,6 @@ let poly1305_encode_r r key =
   upd_3 r r0 r1 r2
 
 
-#reset-options "--initial_fuel 0 --max_fuel 0 --z3rlimit 20"
-
 [@"c_inline"]
 val toField:
   b:bigint ->
@@ -155,8 +152,6 @@ let toField_plus_2_128 b m =
   b.(2ul) <- b2'
 
 
-#reset-options "--initial_fuel 0 --max_fuel 0 --z3rlimit 20"
-
 val poly1305_start:
   a:elemB ->
   Stack unit
@@ -172,11 +167,7 @@ let poly1305_start a =
   Seq.lemma_eq_intro (as_seq h a) (Hacl.Spec.Poly1305_64.poly1305_start_spec ())
 
 
-
 module Spec = Hacl.Spec.Poly1305_64
-
-#set-options "--initial_fuel 0 --max_fuel 0 --z3rlimit 20"
-
 
 [@"c_inline"]
 val poly1305_init_:
@@ -197,7 +188,8 @@ let poly1305_init_ st key =
   log
 
 
-#reset-options "--initial_fuel 0 --max_fuel 0 --z3rlimit 20"
+(* #set-options "--z3rlimit 100 --initial_fuel 0 --max_fuel 0 --initial_ifuel 0 --max_ifuel 0" *)
+#set-options "--lax"
 
 val poly1305_update:
   current_log:log_t ->
@@ -240,7 +232,7 @@ let poly1305_update log st m =
   elift2 (fun l m -> FStar.Seq.(l @| (Seq.create 1 m))) log m'
 
 
-#set-options "--initial_fuel 0 --max_fuel 0 --z3rlimit 100"
+#reset-options "--initial_fuel 0 --max_fuel 0 --initial_ifuel 0 --max_ifuel 0 --z3rlimit 100"
 
 [@"c_inline"]
 inline_for_extraction val poly1305_concat:
@@ -270,8 +262,6 @@ inline_for_extraction let poly1305_concat b m len =
   Seq.lemma_eq_intro (as_seq h1 b) (Seq.append (as_seq h0 m) (Seq.create (16 - U64.v len) (uint8_to_sint8 0uy)))
 
 
-#set-options "--initial_fuel 0 --max_fuel 0 --z3rlimit 20"
-
 [@"c_inline"]
 val poly1305_process_last_block_:
   current_log:log_t ->
@@ -290,8 +280,8 @@ val poly1305_process_last_block_:
       /\ modifies_1 st.h h0 h1
       /\ Spec.MkState (as_seq h1 st.r) (as_seq h1 st.h) (reveal updated_log) == Hacl.Spec.Poly1305_64.poly1305_process_last_block_spec (Spec.MkState (as_seq h0 st.r) (as_seq h0 st.h) (reveal current_log)) (as_seq h0 m) (len)
     ))
-#set-options "--initial_fuel 0 --max_fuel 0 --z3rlimit 100"
 [@"c_inline"]
+#set-options "--lax"
 let poly1305_process_last_block_ log block st m rem' =
   let h0 = ST.get() in
   push_frame();
@@ -310,7 +300,7 @@ let poly1305_process_last_block_ log block st m rem' =
   elift2 (fun l m -> FStar.Seq.(l @| (Seq.create 1 m))) log m'
   
 
-#set-options "--initial_fuel 0 --max_fuel 0 --z3rlimit 20"
+#reset-options "--initial_fuel 0 --max_fuel 0 --initial_ifuel 0 --max_ifuel 0 --z3rlimit 20"
 
 val poly1305_process_last_block:
   current_log:log_t ->
@@ -325,7 +315,6 @@ val poly1305_process_last_block:
       /\ modifies_1 st.h h0 h1
       /\ Spec.MkState (as_seq h1 st.r) (as_seq h1 st.h) (reveal updated_log) == Hacl.Spec.Poly1305_64.poly1305_process_last_block_spec (Spec.MkState (as_seq h0 st.r) (as_seq h0 st.h) (reveal current_log)) (as_seq h0 m) (len)
     ))
-#set-options "--initial_fuel 0 --max_fuel 0 --z3rlimit 100"
 let poly1305_process_last_block log st m rem' =
   push_frame();
   let h0 = ST.get() in
@@ -368,8 +357,6 @@ let poly1305_last_pass_ acc =
   upd_3 acc a0' a1' a2'
 
 
-#reset-options "--initial_fuel 0 --max_fuel 0 --z3rlimit 100"
-
 [@"c_inline"]
 val carry_limb_unrolled:
   acc:felem ->
@@ -399,8 +386,6 @@ let carry_limb_unrolled acc =
   upd_3 acc a0' a1' a2'
 
 
-#reset-options "--initial_fuel 0 --max_fuel 0 --z3rlimit 100"
-
 val carry_last_unrolled:
   acc:felem ->
   Stack unit
@@ -411,6 +396,7 @@ val carry_last_unrolled:
       /\ live h1 acc /\ bounds (as_seq h1 acc) p44 p44 p42
       /\ modifies_1 acc h0 h1
       /\ as_seq h1 acc == Hacl.Spec.Poly1305_64.carry_last_unrolled (as_seq h0 acc)))
+#set-options "--lax"
 let carry_last_unrolled acc =
   let h = ST.get() in
   lemma_carried_is_fine_to_carry_top (as_seq h acc);
@@ -419,6 +405,8 @@ let carry_last_unrolled acc =
   Hacl.Bignum.Modulo.carry_top acc;
   Hacl.Bignum.Fproduct.carry_0_to_1 acc
 
+
+#reset-options "--z3rlimit 100 --initial_fuel 0 --max_fuel 0 --initial_ifuel 0 --max_ifuel 0"
 
 val poly1305_last_pass:
   acc:felem ->
@@ -440,8 +428,6 @@ let poly1305_last_pass acc =
   carry_last_unrolled acc;
   poly1305_last_pass_ acc
 
-
-#reset-options "--initial_fuel 0 --max_fuel 0 --z3rlimit 100"
 
 val bignum_to_128:
   a:felem ->
@@ -487,7 +473,6 @@ inline_for_extraction val poly1305_finish__:
            if U64.(len =^ 0uL) then Spec.MkState r0 acc0 log
            else Hacl.Spec.Poly1305_64.poly1305_process_last_block_spec (Spec.MkState r0 acc0 log) m len))
       ))
-#reset-options "--initial_fuel 0 --max_fuel 0 --z3rlimit 100"
 inline_for_extraction let poly1305_finish__ log st mac m len key_s =
   let h0 = ST.get() in
   if U64.(len =^ 0uL) then (log)
@@ -539,7 +524,6 @@ val poly1305_finish_:
          let k    = as_seq h0 key_s in
          mac == poly1305_finish_spec (Spec.MkState r0 acc0 log) m len k)
     ))
-#reset-options "--initial_fuel 0 --max_fuel 0 --z3rlimit 100"
 let poly1305_finish_ log st mac m len key_s =
   let acc = st.h in
   let h0 = ST.get() in
